fix rsa

code/experimental/rsa/Hacl.Impl.RSA.fst
@@ -17,310 +17,237 @@ open Hacl.Impl.Multiplication
 
 module Buffer = Spec.Lib.IntBuf
 
-inline_for_extraction let hLen:size_t = size 32
+inline_for_extraction
+let hLen:size_t = size 32
 
 val xor_bytes:
-    #len:size_nat ->
-    clen:size_t{v clen == len} ->
-    b1:lbytes len ->
-    b2:lbytes len -> Stack unit
-    (requires (fun h -> live h b1 /\ live h b2))
-    (ensures (fun h0 _ h1 -> preserves_live h0 h1 /\ modifies1 b1 h0 h1))
-    [@"c_inline"]
+  #len:size_nat -> clen:size_t{v clen == len} ->
+  b1:lbytes len -> b2:lbytes len -> Stack unit
+  (requires (fun h -> live h b1 /\ live h b2 /\ disjoint b1 b2))
+  (ensures (fun h0 _ h1 -> preserves_live h0 h1 /\ modifies1 b1 h0 h1))
+  [@"c_inline"]
 let xor_bytes #len clen b1 b2 = map2 #uint8 #uint8 #len clen (fun x y -> logxor #U8 x y) b1 b2
-  
-val pss_encode_:
-    #sLen:size_nat -> #msgLen:size_nat -> #emLen:size_nat ->
-    ssLen:size_t{v ssLen == sLen /\ sLen + v hLen + 8 < max_size_t} ->
-    salt:lbytes sLen ->
-    mmsgLen:size_t{v mmsgLen == msgLen} -> msg:lbytes msgLen ->
-    eemLen:size_t{v eemLen == emLen /\  emLen - sLen - v hLen - 2 >= 0} ->
-    em:lbytes emLen -> Stack unit
-    (requires (fun h -> live h salt /\ live h msg /\ live h em /\ 
-	              disjoint msg salt /\ disjoint em msg /\ disjoint em salt))
-    (ensures (fun h0 _ h1 -> preserves_live h0 h1 /\ modifies1 em h0 h1))
-    #reset-options "--z3rlimit 150 --max_fuel 0 --max_ifuel 0"
-    [@"c_inline"]
-let pss_encode_ #sLen #msgLen #emLen ssLen salt mmsgLen msg eemLen em =
-    let m1_size:size_t = add #SIZE (add #SIZE (size 8) hLen) ssLen in
-    assert_norm (v m1_size < max_size_t);
-    let db_size:size_t = sub #SIZE (sub #SIZE eemLen hLen) (size 1) in
-    
-    assume (sLen + v hLen + 8 + 2 * emLen < max_size_t);
-    assume (4 + 2 * v hLen + v hLen * v (blocks db_size hLen) < max_size_t);
-    let stLen:size_t = add #SIZE (add #SIZE (add #SIZE (add #SIZE hLen m1_size) hLen) db_size) db_size in
 
-    alloc #uint8 #unit #(v stLen) stLen (u8 0) [BufItem salt; BufItem msg] [BufItem em]
-    (fun h0 _ h1 -> True)
-    (fun st ->
-       let mHash = Buffer.sub #uint8 #(v stLen) #(v hLen) st (size 0) hLen in
-       let m1 = Buffer.sub #uint8 #(v stLen) #(v m1_size) st hLen m1_size in
-       let m1Hash = Buffer.sub #uint8 #(v stLen) #(v hLen) st (add #SIZE hLen m1_size) hLen in
-       let db = Buffer.sub #uint8 #(v stLen) #(v db_size) st (add #SIZE (add #SIZE hLen m1_size) hLen) db_size in
-       let dbMask = Buffer.sub #uint8 #(v stLen) #(v db_size) st (add #SIZE (add #SIZE (add #SIZE hLen m1_size) hLen) db_size) db_size in
-       disjoint_sub_lemma1 st msg (size 0) hLen;
-       hash_sha256 mHash mmsgLen msg;
-    
-       let m1' = Buffer.sub #uint8 #(v m1_size) #(v hLen) m1 (size 8) hLen in
-       copy hLen mHash m1';
-       let m1' = Buffer.sub #uint8 #(v m1_size) #sLen m1 (add #SIZE (size 8) hLen) ssLen in
-       copy ssLen salt m1';
-       hash_sha256 m1Hash m1_size m1;
-       
-       let last_before_salt = sub #SIZE (sub #SIZE db_size ssLen) (size 1) in
-       db.(last_before_salt) <- u8 1;
-       let db' = Buffer.sub #uint8 #(v db_size) #sLen db (last_before_salt +! size 1) ssLen in
-       copy ssLen salt db';
-    
-       //mgf_sha256 m1Hash db_size dbMask;
-       mgf_sha256 #(v hLen) #(v db_size) hLen m1Hash db_size dbMask;
-       xor_bytes db_size db dbMask;
-       
-       let em' = Buffer.sub #uint8 #emLen #(v db_size) em (size 0) db_size in
-       copy db_size db em';
-       let em' = Buffer.sub #uint8 #emLen #(v hLen) em db_size hLen in
-       copy hLen m1Hash em';
-       em.(sub #SIZE eemLen (size 1)) <- u8 0xbc
-    )
-		
 val pss_encode:
-    #sLen:size_nat -> #msgLen:size_nat -> #emLen:size_nat ->
-    msBits:size_t{v msBits < 8} ->
-    ssLen:size_t{v ssLen == sLen /\ sLen + v hLen + 8 < max_size_t} -> salt:lbytes sLen ->
-    mmsgLen:size_t{v mmsgLen == msgLen /\ msgLen < pow2 61} -> msg:lbytes msgLen ->
-    eemLen:size_t{v eemLen == emLen /\ emLen - sLen - v hLen - 3 >= 0} ->
-    em:lbytes emLen -> Stack unit
-    (requires (fun h -> live h salt /\ live h msg /\ live h em /\ disjoint msg salt /\ disjoint em msg /\ disjoint em salt))
-    (ensures (fun h0 _ h1 -> preserves_live h0 h1 /\ modifies1 em h0 h1))
-    #reset-options "--z3rlimit 50 --max_fuel 0"
-    [@"c_inline"]
-let pss_encode #sLen #msgLen #emLen msBits ssLen salt mmsgLen msg eemLen em =
-    if (msBits =. size 0)
-    then begin
-	let em' = Buffer.sub #uint8 #emLen #(emLen - 1) em (size 1) (sub #SIZE eemLen (size 1)) in
-	disjoint_sub_lemma1 em msg (size 1) (sub #SIZE eemLen (size 1));
-	disjoint_sub_lemma1 em salt (size 1) (sub #SIZE eemLen (size 1));
-	pss_encode_ ssLen salt mmsgLen msg (sub #SIZE eemLen (size 1)) em' end
-    else begin
-	pss_encode_ ssLen salt mmsgLen msg eemLen em;
-	let shift' = sub #SIZE (size 8) msBits in
-	em.(size 0) <- em.(size 0) &. (shift_right #U8 (u8 0xff) (size_to_uint32 shift'))
-    end
+  #sLen:size_nat -> #msgLen:size_nat -> #emLen:size_nat ->
+  ssLen:size_t{v ssLen = sLen /\ 8 + v hLen + sLen < max_size_t} -> salt:lbytes sLen ->
+  mmsgLen:size_t{v mmsgLen = msgLen} -> msg:lbytes msgLen ->
+  emBits:size_t{v emBits > 0 /\ emLen = v (blocks emBits (size 8)) /\ v hLen + sLen + 2 <= v (blocks emBits (size 8))} ->
+  em:lbytes emLen -> Stack unit
+  (requires (fun h -> live h salt /\ live h msg /\ live h em /\
+		    disjoint msg salt /\ disjoint em msg /\ disjoint em salt))
+  (ensures (fun h0 _ h1 -> preserves_live h0 h1 /\ modifies1 em h0 h1))
+  [@"c_inline"]
+  #reset-options "--z3rlimit 50 --max_fuel 0 --max_ifuel 0"
+let pss_encode #sLen #msgLen #emLen ssLen salt mmsgLen msg emBits em =
+  let (emLen:size_t{v emLen > 0}) = blocks emBits (size 8) in
+  let (msBits:size_t{v msBits < 8}) = emBits %. (size 8) in
 
-val pss_verify_:
-    #sLen:size_nat -> #msgLen:size_nat -> #emLen:size_nat ->
-    ssLen:size_t{v ssLen == sLen /\ sLen + v hLen + 8 < max_size_t} ->
-    msBits:size_t{v msBits < 8} ->
-    eemLen:size_t{v eemLen == emLen /\ emLen - sLen - v hLen - 2 >= 0} ->
-    em:lbytes emLen ->
-    mmsgLen:size_t{v mmsgLen == msgLen} ->
-    msg:lbytes msgLen -> Stack bool
-    (requires (fun h -> live h em /\ live h msg /\ disjoint em msg))
-    (ensures (fun h0 _ h1 -> preserves_live h0 h1 /\ modifies0 h0 h1))
-    #reset-options "--z3rlimit 150 --max_fuel 0 --max_ifuel 0"
-    [@"c_inline"]
-let pss_verify_ #sLen #msgLen #emLen ssLen msBits eemLen em mmsgLen msg =
-    let pad_size:size_t = sub #SIZE (sub #SIZE (sub #SIZE eemLen ssLen) hLen) (size 1) in
-    let db_size:size_t = sub #SIZE (sub #SIZE eemLen hLen) (size 1) in
-    assert_norm (v db_size < max_size_t);
-    let m1_size:size_t = add #SIZE (add #SIZE (size 8) hLen) ssLen in
-    assert_norm (v m1_size < max_size_t);
-    
-    assume (2 * emLen +  8 + v hLen  < max_size_t);
-    assume (4 + 2 * v hLen + v hLen * v (blocks db_size hLen) < max_size_t);
-    let stLen = add #SIZE (add #SIZE (add #SIZE (add #SIZE hLen pad_size) db_size) m1_size) hLen in
-    
-    alloc #uint8 #bool #(v stLen) stLen (u8 0) [BufItem em; BufItem msg] []
-    (fun h0 _ h1 -> True)
-    (fun st ->
-       let mHash = Buffer.sub #uint8 #(v stLen) #(v hLen) st (size 0) hLen in
-       let pad2 = Buffer.sub #uint8 #(v stLen) #(v pad_size) st hLen pad_size in
-       let dbMask = Buffer.sub #uint8 #(v stLen) #(v db_size) st (add #SIZE hLen pad_size) db_size in
-       let m1 = Buffer.sub #uint8 #(v stLen) #(v m1_size) st (add #SIZE (add #SIZE hLen pad_size) db_size) m1_size in
-       let m1Hash' = Buffer.sub #uint8 #(v stLen) #(v hLen) st (add #SIZE (add #SIZE (add #SIZE hLen pad_size) db_size) m1_size) hLen in
-       
-       disjoint_sub_lemma1 st msg (size 0) hLen;
-       hash_sha256 mHash mmsgLen msg;
-       
-       pad2.(sub #SIZE pad_size (size 1)) <- u8 0x01;
-       let maskedDB = Buffer.sub #uint8 #emLen #(v db_size) em (size 0) db_size in
-       let m1Hash = Buffer.sub #uint8 #emLen #(v hLen) em db_size hLen in
-       //mgf_sha256 m1Hash db_size dbMask;
-       mgf_sha256 #(v hLen) #(v db_size) hLen m1Hash db_size dbMask;
-       xor_bytes db_size dbMask maskedDB;
-    
-       (if (msBits >. size 0) then begin
-	 let shift' = sub #SIZE (size 8) msBits in
-	 dbMask.(size 0) <- dbMask.(size 0) &. (shift_right #U8 (u8 0xff) (size_to_uint32 shift')) end);
+  let m1Len:size_t = add #SIZE (add #SIZE (size 8) hLen) ssLen in
+  let (dbLen:size_t{v dbLen > 0}) = sub #SIZE (sub #SIZE emLen hLen) (size 1) in
+  //st = [hash(msg); m1; hash(m1); db; dbMask]
+  assume (2 * v hLen + 4 + v (blocks dbLen hLen) * v hLen < pow2 32); //for mgf
+  assume (v hLen + sLen + 6 + 2 * v emLen < max_size_t);
+  let stLen:size_t = add #SIZE (add #SIZE (add #SIZE (add #SIZE hLen m1Len) hLen) dbLen) dbLen in
 
-       //let pad = Buffer.sub #uint8 #stLen #(v pad_size) st (add #SIZE hLen pad_size) pad_size in
-       let pad = Buffer.sub #uint8 #(v db_size) #(v pad_size) dbMask (size 0) pad_size in
-       let salt = Buffer.sub #uint8 #(v db_size) #sLen dbMask pad_size ssLen in
+  alloc #uint8 #unit #(v stLen) stLen (u8 0) [BufItem salt; BufItem msg] [BufItem em]
+  (fun h0 _ h1 -> True)
+  (fun st ->
+    let mHash = Buffer.sub #uint8 #(v stLen) #(v hLen) st (size 0) hLen in
+    let m1 = Buffer.sub #uint8 #(v stLen) #(v m1Len) st hLen m1Len in
+    let m1Hash = Buffer.sub #uint8 #(v stLen) #(v hLen) st (add #SIZE hLen m1Len) hLen in
+    let db = Buffer.sub #uint8 #(v stLen) #(v dbLen) st (add #SIZE (add #SIZE hLen m1Len) hLen) dbLen in
+    let dbMask = Buffer.sub #uint8 #(v stLen) #(v dbLen) st (add #SIZE (add #SIZE (add #SIZE hLen m1Len) hLen) dbLen) dbLen in
 
-       assume (disjoint pad pad2);
-       let res =
-	 if not (eq_b pad_size pad pad2) then false
-	 else begin
-	     let m1' = Buffer.sub #uint8 #(v m1_size) #(v hLen) m1 (size 8) hLen in
-	     copy hLen mHash m1';
-	     let m1' = Buffer.sub #uint8 #(v m1_size) #sLen m1 (add #SIZE (size 8) hLen) ssLen in
-	     copy ssLen salt m1';
-	     hash_sha256 m1Hash' m1_size m1;
-	     disjoint_sub_lemma3 em st db_size hLen (add #SIZE (add #SIZE (add #SIZE hLen pad_size) db_size) m1_size) hLen;
-	     eq_b hLen m1Hash m1Hash'
-	end in
-      res
-    )
+    hash_sha256 mHash mmsgLen msg;
+    let m1_hash = Buffer.sub #uint8 #(v m1Len) #(v hLen) m1 (size 8) hLen in
+    copy hLen mHash m1_hash;
+    let m1_salt = Buffer.sub #uint8 #(v m1Len) #sLen m1 (add #SIZE (size 8) hLen) ssLen in
+    copy ssLen salt m1_salt;
+    hash_sha256 m1Hash m1Len m1;
+
+    assert (0 <= v dbLen - sLen - 1);
+    let last_before_salt = sub #SIZE (sub #SIZE dbLen ssLen) (size 1) in
+    db.(last_before_salt) <- u8 1;
+    let db_salt = Buffer.sub #uint8 #(v dbLen) #sLen db (add #SIZE last_before_salt (size 1)) ssLen in
+    copy ssLen salt db_salt;
+    mgf_sha256 #(v hLen) #(v dbLen) hLen m1Hash dbLen dbMask;
+    xor_bytes dbLen db dbMask;
+
+    (if (msBits >. size 0) then begin
+      let shift_bits = sub #SIZE (size 8) msBits in
+      assert (0 < v shift_bits /\ v shift_bits < 8);
+      db.(size 0) <- db.(size 0) &. (shift_right #U8 (u8 0xff) (size_to_uint32 shift_bits))
+    end);
+
+    let em_db = Buffer.sub #uint8 #(v emLen) #(v dbLen) em (size 0) dbLen in
+    copy dbLen db em_db;
+    let em_hash = Buffer.sub #uint8 #(v emLen) #(v hLen) em dbLen hLen in
+    copy hLen m1Hash em_hash;
+    em.(sub #SIZE emLen (size 1)) <- u8 0xbc
+  )
 
 val pss_verify:
-    #sLen:size_nat -> #msgLen:size_nat -> #emLen:size_nat ->
-    ssLen:size_t{v ssLen == sLen /\ sLen + v hLen + 8 < max_size_t} ->
-    msBits:size_t{v msBits < 8} ->
-    eemLen:size_t{v eemLen == emLen /\ emLen - sLen - v hLen - 2 >= 0} ->
-    em:lbytes emLen ->
-    mmsgLen:size_t{v mmsgLen == msgLen} -> msg:lbytes msgLen -> Stack bool
-    (requires (fun h -> live h em /\ live h msg /\ disjoint em msg))
-    (ensures (fun h0 _ h1 -> preserves_live h0 h1 /\ modifies0 h0 h1))
-    #reset-options "--z3rlimit 50 --max_fuel 0 --max_ifuel 0"
-    [@"c_inline"]
-let pss_verify #sLen #msgLen #emLen ssLen msBits eemLen em mmsgLen msg =
-    let h0 = FStar.HyperStack.ST.get() in
-    let em_0 = em.(size 0) &. (shift_left #U8 (u8 0xff) (size_to_uint32 msBits)) in
-    let em_last = em.(sub #SIZE eemLen (size 1)) in
+  #msgLen:size_nat -> #emLen:size_nat ->
+  sLen:size_t{8 + v hLen + v sLen < max_size_t} ->
+  mmsgLen:size_t{v mmsgLen = msgLen} -> msg:lbytes msgLen ->
+  emBits:size_t{v emBits > 0 /\ emLen = v (blocks emBits (size 8)) /\ v hLen + v sLen + 2 <= v (blocks emBits (size 8))} -> // <- check the last condition before calling this function!
+  em:lbytes emLen -> Stack bool
+  (requires (fun h -> live h msg /\ live h em /\ disjoint em msg))
+  (ensures (fun h0 _ h1 -> preserves_live h0 h1 /\ modifies0 h0 h1))
+  [@"c_inline"]
+  #reset-options "--z3rlimit 50 --max_fuel 0 --max_ifuel 0"
+let pss_verify #msgLen #emLen sLen mmsgLen msg emBits em =
+  let (emLen:size_t{v emLen > 0}) = blocks emBits (size 8) in
+  let (msBits:size_t{v msBits < 8}) = emBits %. (size 8) in
 
-    let res = 
-      if not ((eq_u8 em_0 (u8 0)) && (eq_u8 em_last (u8 0xbc)))
-      then false
-      else begin
-	 let eemLen1 = if msBits =. size 0 then sub #SIZE eemLen (size 1) else eemLen in
-	 let em1:lbytes (v eemLen1) =
-	     if msBits =. size 0 then begin
-	       let em' = Buffer.sub em (size 1) eemLen1 in
-	       disjoint_sub_lemma1 em msg (size 1) eemLen1;
-	       em' end
-	     else em in
-	 if (eemLen1 <. add #SIZE (add #SIZE ssLen hLen) (size 2)) then false
-	 else pss_verify_ #sLen #msgLen #(v eemLen1) ssLen msBits eemLen1 em1 mmsgLen msg
-      end in
-    let h1 = FStar.HyperStack.ST.get() in
-    assume (modifies0 h0 h1);
-    res
+  let em_0 = if (msBits >. size 0) then em.(size 0) &. (shift_left #U8 (u8 0xff) (size_to_uint32 msBits)) else u8 0 in
+  let em_last = em.(sub #SIZE emLen (size 1)) in
+
+  let padLen:size_t = sub #SIZE (sub #SIZE (sub #SIZE emLen sLen) hLen) (size 1) in
+  let dbLen:size_t = sub #SIZE (sub #SIZE emLen hLen) (size 1) in
+  let m1Len:size_t = add #SIZE (add #SIZE (size 8) hLen) sLen in
+  assume (4 + 2 * v hLen + v hLen * v (blocks dbLen hLen) < max_size_t);
+  //st = [hash(msg); pad; dbMask; m1; hash(m1)]
+  let stLen = add #SIZE (add #SIZE (add #SIZE (add #SIZE hLen padLen) dbLen) m1Len) hLen in
+  alloc #uint8 #bool #(v stLen) stLen (u8 0) [BufItem em; BufItem msg] []
+  (fun h0 _ h1 -> True)
+  (fun st ->
+    if not ((eq_u8 em_0 (u8 0)) && (eq_u8 em_last (u8 0xbc))) then false
+    else begin
+      let mHash = Buffer.sub #uint8 #(v stLen) #(v hLen) st (size 0) hLen in
+      let pad2 = Buffer.sub #uint8 #(v stLen) #(v padLen) st hLen padLen in
+      let dbMask = Buffer.sub #uint8 #(v stLen) #(v dbLen) st (add #SIZE hLen padLen) dbLen in
+      let m1 = Buffer.sub #uint8 #(v stLen) #(v m1Len) st (add #SIZE (add #SIZE hLen padLen) dbLen) m1Len in
+      let m1Hash' = Buffer.sub #uint8 #(v stLen) #(v hLen) st (sub #SIZE stLen hLen) hLen in
+
+      let maskedDB = Buffer.sub #uint8 #(v emLen) #(v dbLen) em (size 0) dbLen in
+      let m1Hash = Buffer.sub #uint8 #(v emLen) #(v hLen) em dbLen hLen in
+
+      hash_sha256 mHash mmsgLen msg;
+
+      mgf_sha256 #(v hLen) #(v dbLen) hLen m1Hash dbLen dbMask;
+      xor_bytes dbLen dbMask maskedDB;
+      (if (msBits >. size 0) then begin
+        let shift_bits = sub #SIZE (size 8) msBits in
+        dbMask.(size 0) <- dbMask.(size 0) &. (shift_right #U8 (u8 0xff) (size_to_uint32 shift_bits))
+      end);
+
+      pad2.(sub #SIZE padLen (size 1)) <- u8 0x01;
+      let pad = Buffer.sub #uint8 #(v dbLen) #(v padLen) dbMask (size 0) padLen in
+      let salt = Buffer.sub #uint8 #(v dbLen) #(v sLen) dbMask padLen sLen in
+
+      let m1_hash = Buffer.sub #uint8 #(v m1Len) #(v hLen) m1 (size 8) hLen in
+      copy hLen mHash m1_hash;
+      let m1_salt = Buffer.sub #uint8 #(v m1Len) #(v sLen) m1 (add #SIZE (size 8) hLen) sLen in
+      copy sLen salt m1_salt;
+      hash_sha256 m1Hash' m1Len m1;
+
+      if not (eq_b padLen pad pad2) then false
+      else eq_b hLen m1Hash m1Hash'
+    end
+  )
 
 val rsa_sign:
-    #sLen:size_nat -> #msgLen:size_nat -> #nLen:size_nat ->
-    pow2_i:size_t{6 * nLen + 4 * v pow2_i < max_size_t /\ nLen <= v pow2_i /\ nLen + 1 < 2 * v pow2_i} ->
-    modBits:size_t{0 < v modBits /\ nLen = v (bits_to_bn modBits)} ->
-    eBits:size_t{0 < v eBits /\ v eBits <= v modBits} ->
-    dBits:size_t{0 < v dBits /\ v dBits <= v modBits} ->
-    pLen:size_t -> qLen:size_t{nLen + v (bits_to_bn eBits) + v (bits_to_bn dBits) + v pLen + v qLen < max_size_t} ->
-    skey:lbignum (nLen + v (bits_to_bn eBits) + v (bits_to_bn dBits) + v pLen + v qLen) ->
-    rBlind:uint64 ->
-    ssLen:size_t{v ssLen == sLen /\ sLen + v hLen + 8 < max_size_t /\ v (blocks modBits (size 8)) - sLen - v hLen - 3 >= 0} -> salt:lbytes sLen ->
-    mmsgLen:size_t{v mmsgLen == msgLen /\ msgLen < pow2 61} -> msg:lbytes msgLen ->
-    sgnt:lbytes (v (blocks modBits (size 8))) -> Stack unit
-    (requires (fun h -> live h salt /\ live h msg /\ live h sgnt /\ live h skey /\
-	              disjoint msg salt /\ disjoint msg sgnt /\ disjoint sgnt salt))
-    (ensures (fun h0 _ h1 -> preserves_live h0 h1 /\ modifies1 sgnt h0 h1))
+  #sLen:size_nat -> #msgLen:size_nat -> #nLen:size_nat ->
+  pow2_i:size_t -> modBits:size_t{0 < v modBits /\ nLen = v (blocks modBits (size 64))} ->
+  eBits:size_t{0 < v eBits /\ v eBits <= v modBits} -> dBits:size_t{0 < v dBits /\ v dBits <= v modBits} ->
+  pLen:size_t -> qLen:size_t{nLen + v (blocks eBits (size 64)) + v (blocks dBits (size 64)) + v pLen + v qLen < max_size_t} ->
+  skey:lbignum (nLen + v (blocks eBits (size 64)) + v (blocks dBits (size 64)) + v pLen + v qLen) -> rBlind:uint64 ->
+  ssLen:size_t{v ssLen == sLen /\ sLen + v hLen + 8 < max_size_t /\ v (blocks modBits (size 8)) - sLen - v hLen - 2 >= 0} -> salt:lbytes sLen ->
+  mmsgLen:size_t{v mmsgLen == msgLen} -> msg:lbytes msgLen -> sgnt:lbytes (v (blocks modBits (size 8))) -> Stack unit
+  (requires (fun h -> live h salt /\ live h msg /\ live h sgnt /\ live h skey /\
+	            disjoint msg salt /\ disjoint msg sgnt /\ disjoint sgnt salt))
+  (ensures (fun h0 _ h1 -> preserves_live h0 h1 /\ modifies1 sgnt h0 h1))
 
-    #reset-options "--z3rlimit 1000 --max_fuel 0 --max_ifuel 0"
-     
 let rsa_sign #sLen #msgLen #nLen pow2_i modBits eBits dBits pLen qLen skey rBlind ssLen salt mmsgLen msg sgnt =
-    let k = blocks modBits (size 8) in
-    let msBits = (sub #SIZE modBits (size 1)) %. size 8 in
+  let nLen = blocks modBits (size 64) in
+  let eLen = blocks eBits (size 64) in
+  let dLen = blocks dBits (size 64) in
+  let skeyLen:size_t = add #SIZE (add #SIZE (add #SIZE (add #SIZE nLen eLen) dLen) pLen) qLen in
 
-    //let nLen = bits_to_bn modBits in
-    let nLen = get_size_nat k in
-    let eLen = bits_to_bn eBits in
-    let dLen = bits_to_bn dBits in
-    let skeyLen:size_t = add #SIZE (add #SIZE (add #SIZE (add #SIZE nLen eLen) dLen) pLen) qLen in
-    
-    let n = Buffer.sub #uint64 #(v skeyLen) #(v nLen) skey (size 0) nLen in
-    let e = Buffer.sub #uint64 #(v skeyLen) #(v eLen) skey nLen eLen in
-    let d = Buffer.sub #uint64 #(v skeyLen) #(v dLen) skey (add #SIZE nLen eLen) dLen in
-    let p = Buffer.sub #uint64 #(v skeyLen) #(v pLen) skey (add #SIZE (add #SIZE nLen eLen) dLen) pLen in
-    let q = Buffer.sub #uint64 #(v skeyLen) #(v qLen) skey (add #SIZE ((add #SIZE (add #SIZE nLen eLen) dLen)) pLen) qLen in
-    
-    assume (2 * v nLen + 2 * (v pLen + v qLen) + 1 < max_size_t);   
-    //assume (8 * v nLen < max_size_t);
-    let n2Len = add #SIZE nLen nLen in
-    let pqLen = add #SIZE pLen qLen in
-    let stLen:size_t = add #SIZE n2Len (add #SIZE (add #SIZE pqLen pqLen) (size 1)) in
-    
-    alloc #uint8 #unit #(v k) k (u8 0) [BufItem skey; BufItem msg; BufItem salt] [BufItem sgnt]
-    (fun h0 _ h1 -> True)
-    (fun em -> 
-       pss_encode msBits ssLen salt mmsgLen msg k em;
-      	
-       alloc #uint64 #unit #(v stLen) stLen (u64 0) [BufItem skey; BufItem em] [BufItem sgnt]
-       (fun h0 _ h1 -> True)
-       (fun tmp ->
-           let m = Buffer.sub #uint64 #(v stLen) #(v nLen) tmp (size 0) nLen in
-           let s = Buffer.sub #uint64 #(v stLen) #(v nLen) tmp nLen nLen in
-           let phi_n = Buffer.sub #uint64 #(v stLen) #(v pqLen) tmp n2Len pqLen in
-           let p1 = Buffer.sub #uint64 #(v stLen) #(v pLen) tmp (add #SIZE n2Len pqLen) pLen in
-           let q1 = Buffer.sub #uint64 #(v stLen) #(v qLen) tmp (add #SIZE (add #SIZE n2Len pqLen) pLen) qLen in
-           let dLen':size_t = add #SIZE (add #SIZE pLen qLen) (size 1) in
-           let d' = Buffer.sub #uint64 #(v stLen) #(v dLen') tmp (add #SIZE n2Len pqLen) dLen' in admit();
-           assume (disjoint m em);
-           text_to_nat k em m;
-           bn_sub_u64 pLen p (u64 1) p1; // p1 = p - 1
-           bn_sub_u64 qLen q (u64 1) q1; // q1 = q - 1
-           bn_mul pLen p1 qLen q1 phi_n; // phi_n = p1 * q1
-           bn_mul_u64 pqLen phi_n rBlind d'; //d' = phi_n * rBlind
-           assume (v dLen <= v dLen' /\ v dLen' * 64 < max_size_t);
-           bn_add dLen' d' dLen d d'; //d' = d' + d
-           assume (v nLen = v (bits_to_bn modBits));
-           mod_exp pow2_i modBits nLen n m (mul #SIZE dLen' (size 64)) d' s;
-           nat_to_text k s sgnt
-        )
-    )
+  let n = Buffer.sub #uint64 #(v skeyLen) #(v nLen) skey (size 0) nLen in
+  let e = Buffer.sub #uint64 #(v skeyLen) #(v eLen) skey nLen eLen in
+  let d = Buffer.sub #uint64 #(v skeyLen) #(v dLen) skey (add #SIZE nLen eLen) dLen in
+  let p = Buffer.sub #uint64 #(v skeyLen) #(v pLen) skey (add #SIZE (add #SIZE nLen eLen) dLen) pLen in
+  let q = Buffer.sub #uint64 #(v skeyLen) #(v qLen) skey (add #SIZE ((add #SIZE (add #SIZE nLen eLen) dLen)) pLen) qLen in
 
-val rsa_verify:
-    #sLen:size_nat -> #msgLen:size_nat -> #nLen:size_nat ->
-    pow2_i:size_t{6 * nLen + 4 * v pow2_i < max_size_t /\ nLen <= v pow2_i /\ nLen + 1 < 2 * v pow2_i} ->
-    modBits:size_t{0 < v modBits /\ nLen = v (bits_to_bn modBits)} ->
-    eBits:size_t{0 < v eBits /\ v eBits <= v modBits /\ nLen + v (bits_to_bn eBits) < max_size_t} ->
-    pkey:lbignum (nLen + v (bits_to_bn eBits)) ->
-    ssLen:size_t{v ssLen == sLen /\ sLen + v hLen + 8 < max_size_t /\ v (blocks modBits (size 8)) - sLen - v hLen - 3 >= 0} ->
-    sgnt:lbytes (v (blocks modBits (size 8))) ->
-    mmsgLen:size_t{v mmsgLen == msgLen /\ msgLen < pow2 61} -> msg:lbytes msgLen -> Stack bool
-    (requires (fun h -> live h msg /\ live h sgnt /\ live h pkey /\ disjoint msg sgnt))
-    (ensures (fun h0 _ h1 -> preserves_live h0 h1 /\ modifies0 h0 h1))
+  let k = blocks modBits (size 8) in
+  let emBits = sub #SIZE modBits (size 1) in
+  let emLen = blocks emBits (size 8) in
 
-    #reset-options "--z3rlimit 750 --max_fuel 0 --max_ifuel 0"
-    
-let rsa_verify #sLen #msgLen #nLen pow2_i modBits eBits pkey ssLen sgnt mmsgLen msg =
-    let k = blocks modBits (size 8) in
-    let msBits = (sub #SIZE modBits (size 1)) %. size 8 in
-    //let nLen = bits_to_bn modBits in
-    let nLen = get_size_nat k in
-    let eLen = bits_to_bn eBits in
-    let pkeyLen:size_t = add #SIZE nLen eLen in
+  assume (2 * v nLen + 2 * (v pLen + v qLen) + 1 < max_size_t);
+  let n2Len = add #SIZE nLen nLen in
+  let pqLen = add #SIZE pLen qLen in
+  let stLen:size_t = add #SIZE n2Len (add #SIZE (add #SIZE pqLen pqLen) (size 1)) in
 
-    let n = Buffer.sub #uint64 #(v pkeyLen) #(v nLen) pkey (size 0) nLen in
-    let e = Buffer.sub #uint64 #(v pkeyLen) #(v eLen) pkey nLen eLen in
+  alloc #uint8 #unit #(v emLen) emLen (u8 0) [BufItem skey; BufItem msg; BufItem salt] [BufItem sgnt]
+  (fun h0 _ h1 -> True)
+  (fun em ->
+    pss_encode #sLen #msgLen #(v emLen) ssLen salt mmsgLen msg emBits em;
 
-    let n2Len:size_t = add #SIZE nLen nLen in
-
-    alloc #uint64 #bool #(v n2Len) n2Len (u64 0) [BufItem pkey; BufItem msg; BufItem sgnt] []
+    alloc #uint64 #unit #(v stLen) stLen (u64 0) [BufItem skey; BufItem em] [BufItem sgnt]
     (fun h0 _ h1 -> True)
     (fun tmp ->
-        alloc #uint8 #bool #(v k) k (u8 0) [BufItem pkey; BufItem msg; BufItem sgnt] [BufItem tmp]
-        (fun h0 _ h1 -> True)
-	(fun em ->	
-            let m = Buffer.sub #uint64 #(v n2Len) #(v nLen) tmp (size 0) nLen in
-            let s = Buffer.sub #uint64 #(v n2Len) #(v nLen) tmp nLen nLen in
-            disjoint_sub_lemma1 tmp sgnt nLen nLen;
-            text_to_nat k sgnt s;
-	    
-            assume (disjoint s n);
-	    let res = 
-              if (bn_is_less nLen s nLen n) then begin
-                 mod_exp pow2_i modBits nLen n s eBits e m;
-                 disjoint_sub_lemma1 tmp em (size 0) nLen;
-                 nat_to_text k m em;
-                 pss_verify #sLen #msgLen #(v k) ssLen msBits k em mmsgLen msg end
-              else false in admit();
-            res
-       )
+      let m = Buffer.sub #uint64 #(v stLen) #(v nLen) tmp (size 0) nLen in
+      let s = Buffer.sub #uint64 #(v stLen) #(v nLen) tmp nLen nLen in
+      let phi_n = Buffer.sub #uint64 #(v stLen) #(v pqLen) tmp n2Len pqLen in
+      let p1 = Buffer.sub #uint64 #(v stLen) #(v pLen) tmp (add #SIZE n2Len pqLen) pLen in
+      let q1 = Buffer.sub #uint64 #(v stLen) #(v qLen) tmp (add #SIZE (add #SIZE n2Len pqLen) pLen) qLen in
+      let dLen':size_t = add #SIZE (add #SIZE pLen qLen) (size 1) in
+      let d' = Buffer.sub #uint64 #(v stLen) #(v dLen') tmp (add #SIZE n2Len pqLen) dLen' in
+
+      text_to_nat emLen em m;
+      bn_sub_u64 pLen p (u64 1) p1; // p1 = p - 1
+      bn_sub_u64 qLen q (u64 1) q1; // q1 = q - 1
+      bn_mul pLen p1 qLen q1 phi_n; // phi_n = p1 * q1
+      bn_mul_u64 pqLen phi_n rBlind d'; //d' = phi_n * rBlind
+      assume (v dLen <= v dLen' /\ v dLen' * 64 < max_size_t);
+      bn_add dLen' d' dLen d d'; //d' = d' + d
+      assume (v nLen = v (bits_to_bn modBits));
+      mod_exp pow2_i modBits nLen n m (mul #SIZE dLen' (size 64)) d' s;
+      nat_to_text k s sgnt
     )
+  )
+
+val rsa_verify:
+  #msgLen:size_nat -> #nLen:size_nat ->
+  pow2_i:size_t -> modBits:size_t{0 < v modBits /\ nLen = v (blocks modBits (size 64))} ->
+  eBits:size_t{0 < v eBits /\ v eBits <= v modBits /\ nLen + v (blocks eBits (size 64)) < max_size_t} ->
+  pkey:lbignum (nLen + v (blocks eBits (size 64))) ->
+  sLen:size_t{v sLen + v hLen + 8 < max_size_t /\ v (blocks modBits (size 8)) - v sLen - v hLen - 2 >= 0} ->
+  sgnt:lbytes (v (blocks modBits (size 8))) ->
+  mmsgLen:size_t{v mmsgLen == msgLen} -> msg:lbytes msgLen -> Stack bool
+  (requires (fun h -> live h msg /\ live h sgnt /\ live h pkey /\ disjoint msg sgnt))
+  (ensures (fun h0 _ h1 -> preserves_live h0 h1 /\ modifies0 h0 h1))
+let rsa_verify #msgLen #nLen pow2_i modBits eBits pkey sLen sgnt mmsgLen msg =
+  let nLen = blocks modBits (size 64) in
+  let eLen = blocks eBits (size 64) in
+  let pkeyLen:size_t = add #SIZE nLen eLen in
+
+  let n = Buffer.sub #uint64 #(v pkeyLen) #(v nLen) pkey (size 0) nLen in
+  let e = Buffer.sub #uint64 #(v pkeyLen) #(v eLen) pkey nLen eLen in
+
+  let k = blocks modBits (size 8) in
+  let emBits = sub #SIZE modBits (size 1) in
+  let emLen = blocks emBits (size 8) in
+
+  let n2Len:size_t = add #SIZE nLen nLen in
+
+  alloc #uint64 #bool #(v n2Len) n2Len (u64 0) [BufItem pkey; BufItem msg; BufItem sgnt] []
+  (fun h0 _ h1 -> True)
+  (fun tmp ->
+    alloc #uint8 #bool #(v k) k (u8 0) [BufItem pkey; BufItem msg; BufItem sgnt] [BufItem tmp]
+    (fun h0 _ h1 -> True)
+    (fun em ->
+      let m = Buffer.sub #uint64 #(v n2Len) #(v nLen) tmp (size 0) nLen in
+      let s = Buffer.sub #uint64 #(v n2Len) #(v nLen) tmp nLen nLen in
+      text_to_nat k sgnt s;
+
+      if (bn_is_less nLen s nLen n) then begin
+        mod_exp pow2_i modBits nLen n s eBits e m;
+        nat_to_text emLen m em;
+        pss_verify #msgLen #(v emLen) sLen mmsgLen msg emBits em end
+      else false
+    )
+  )
